Prove most of non-install split

compiler/backend/proofs/clos_interpProofScript.sml
@@ -44,6 +44,161 @@ QED
 
 (* preservation of observable semantics *)
 
+Definition v_ok_def[simp]:
+  (v_ok (Number i) ⇔ T) ∧
+  (v_ok (Word64 w) ⇔ T) ∧
+  (v_ok (Block n vs) ⇔ EVERY v_ok vs) ∧
+  (v_ok (ByteVector ws) ⇔ T) ∧
+  (v_ok (RefPtr n) ⇔ T) ∧
+  (v_ok (Closure loco vs1 env1 n bod1) ⇔
+    ~ has_install bod1 ∧ EVERY v_ok env1 ∧ EVERY v_ok vs1) ∧
+  (v_ok (Recclosure loco vs1 env1 fns1 i) ⇔
+    EVERY v_ok env1 ∧ EVERY v_ok vs1 ∧ i < LENGTH fns1 ∧
+    EVERY ($~ o has_install o SND) fns1)
+Termination
+  WF_REL_TAC ‘measure v_size’ \\ simp[v_size_def]
+End
+
+Definition res_ok_def[simp]:
+  res_ok (Rerr (Rabort _)) = T ∧
+  res_ok (Rerr (Rraise v)) = v_ok v ∧
+  res_ok (Rval v) = EVERY v_ok v
+End
+
+Definition state_rel'_def:
+  state_rel' (s:('c,'ffi) closSem$state) (t:('c,'ffi) closSem$state) <=>
+    (!n. SND (SND (s.compile_oracle n)) = []) ∧
+    s.code = FEMPTY ∧ t.code = FEMPTY ∧
+    t.max_app = s.max_app ∧ 1 <= s.max_app ∧
+    t.clock = s.clock ∧
+    t.ffi = s.ffi ∧
+    s.globals = t.globals ∧ EVERY (OPTION_ALL v_ok) t.globals ∧
+    s.refs = t.refs ∧ FEVERY (λ(k,v). ∀vs. v = ValueArray vs ⇒ EVERY v_ok vs) t.refs ∧
+    s.compile = pure_cc (insert_interp ## I) t.compile ∧
+    t.compile_oracle = pure_co (insert_interp ## I) o s.compile_oracle
+End
+
+Theorem lookup_vars_ok:
+  ∀vs env env'. lookup_vars vs env = SOME env' ∧ EVERY v_ok env ⇒ EVERY v_ok env'
+Proof
+  Induct \\ fs [lookup_vars_def]
+  \\ rw [] \\ gvs [AllCaseEqs()]
+  \\ res_tac \\ fs []
+  \\ gvs [EVERY_EL]
+QED
+
+Triviality state_rel'_clock:
+  state_rel' s t ⇒ t.clock = s.clock
+Proof
+  fs [state_rel'_def]
+QED
+
+Theorem evaluate_change_oracle:
+   (!tmp xs env (s1:('c,'ffi) closSem$state) t1 res s2 n.
+     tmp = (xs,env,s1) ∧
+     (evaluate (xs,env,s1) = (res,s2)) ∧ res <> Rerr (Rabort Rtype_error) ⇒
+     state_rel' s1 t1 ∧ ~(has_install_list xs) ∧ EVERY v_ok env ==>
+     ?t2.
+        (evaluate (xs,env,t1) = (res,t2)) ∧
+        state_rel' s2 t2 ∧ res_ok res) ∧
+   (!loc f args (s:('c,'ffi) closSem$state) res s2 t1.
+       evaluate_app loc f args s = (res,s2) ∧ res <> Rerr (Rabort Rtype_error) ⇒
+       state_rel' s t1 ∧ EVERY v_ok args ∧ v_ok f
+       ⇒
+       ?t2.
+          (evaluate_app loc f args t1 = (res,t2)) ∧
+          state_rel' s2 t2 ∧ res_ok res)
+Proof
+  ho_match_mp_tac evaluate_ind \\ srw_tac[][]
+  \\ fs [has_install_def]
+  >~ [‘evaluate ([],env,t1)’] >-
+   (gvs [evaluate_def])
+  >~ [‘evaluate ((_::_::_),env,t1)’] >-
+   (gvs [evaluate_def,AllCaseEqs()]
+    \\ res_tac \\ gvs []
+    \\ res_tac \\ gvs []
+    \\ imp_res_tac evaluate_SING \\ gvs [])
+  >~ [‘evaluate ([Var _ _],env,t1)’] >-
+    gvs [evaluate_def,AllCaseEqs(),EVERY_EL]
+  >~ [‘evaluate ([If _ _ _ _],env,t1)’] >-
+   (gvs [evaluate_def,AllCaseEqs(),EVERY_EL]
+    \\ res_tac \\ gvs [])
+  >~ [‘evaluate ([Let _ _ _],env,t1)’] >-
+   (gvs [evaluate_def,AllCaseEqs(),EVERY_EL]
+    \\ res_tac \\ gvs [])
+  >~ [‘Tick’] >-
+   (gvs [evaluate_def,AllCaseEqs(),EVERY_EL]
+    >- fs [state_rel'_def]
+    \\ ‘state_rel' (dec_clock 1 s) (dec_clock 1 t1)’ by
+         fs [state_rel'_def,dec_clock_def]
+    \\ res_tac \\ fs []
+    \\ fs [state_rel'_def])
+  >~ [‘evaluate ([Raise _ _],env,t1)’] >-
+   (gvs [evaluate_def,AllCaseEqs(),EVERY_EL]
+    \\ res_tac \\ gvs []
+    \\ imp_res_tac evaluate_SING \\ gvs [])
+  >~ [‘evaluate ([Handle _ _ _],env,t1)’] >-
+   (gvs [evaluate_def,AllCaseEqs(),EVERY_EL]
+    \\ res_tac \\ gvs [])
+  >~ [‘Fn’] >-
+   (gvs [evaluate_def,AllCaseEqs(),state_rel'_def]
+    \\ res_tac \\ gvs [SF ETA_ss]
+    \\ imp_res_tac lookup_vars_ok \\ fs [])
+  >~ [‘Call’] >-
+   (gvs [evaluate_def,AllCaseEqs()]
+    \\ res_tac \\ fs [EXISTS_PROD,PULL_EXISTS]
+    \\ gvs [find_code_def,state_rel'_def])
+  >~ [‘Op’] >-
+   cheat
+  >~ [‘Letrec’] >-
+   (gvs [evaluate_def,AllCaseEqs()]
+    \\ first_x_assum drule
+    \\ impl_tac >-
+     (gvs [EVERY_GENLIST,SF ETA_ss] \\ gvs [EVERY_EL]
+      \\ rw []
+      \\ first_x_assum drule
+      \\ Cases_on ‘EL n fns’ \\ fs []
+      \\ cheat)
+    \\ strip_tac \\ fs []
+    \\ gvs [EVERY_EL] \\ rw [] \\ res_tac \\ gvs [state_rel'_def])
+  >~ [‘App’] >-
+   (gvs [evaluate_def,AllCaseEqs()]
+    \\ res_tac \\ fs [EXISTS_PROD,PULL_EXISTS]
+    \\ res_tac \\ fs []
+    \\ imp_res_tac evaluate_SING \\ gvs [])
+  >~ [‘evaluate_app’] >-
+   (gvs [evaluate_def,AllCaseEqs()]
+    \\ ‘s.max_app = t1.max_app’ by fs [state_rel'_def] \\ fs []
+    \\ TRY (fs [state_rel'_def,dec_clock_def] \\ NO_TAC)
+    >-
+     (fs [state_rel'_def,dec_clock_def]
+      \\ Cases_on ‘f’ \\ gvs [dest_closure_def,AllCaseEqs(),SF ETA_ss]
+      \\ pairarg_tac \\ gvs [dest_closure_def,AllCaseEqs(),SF ETA_ss])
+    \\ gvs [PULL_EXISTS]
+    \\ rename [‘SUC (LENGTH vs)’]
+    \\ ‘state_rel' (dec_clock (SUC (LENGTH vs) − LENGTH rest_args) s)
+                   (dec_clock (SUC (LENGTH vs) − LENGTH rest_args) t1)’ by
+             gvs [dec_clock_def,state_rel'_def]
+    \\ rpt $ first_x_assum drule
+    \\ ‘~has_install exp ∧ EVERY v_ok env ∧ EVERY v_ok rest_args’ by
+     (Cases_on ‘f’ \\ gvs [dest_closure_def,AllCaseEqs(),SF ETA_ss]
+      \\ rpt (pairarg_tac \\ gvs [dest_closure_def,AllCaseEqs(),SF ETA_ss])
+      \\ rpt $ irule_at Any EVERY_TAKE
+      \\ rpt $ irule_at Any EVERY_DROP \\ fs []
+      \\ gvs [EVERY_GENLIST]
+      \\ gvs [EVERY_EL]
+      \\ res_tac
+      \\ qpat_x_assum ‘EL n _ = _’ assume_tac \\ fs [])
+    \\ fs []
+    \\ strip_tac \\ gvs []
+    \\ imp_res_tac state_rel'_clock
+    \\ res_tac \\ fs []
+    \\ first_x_assum $ irule_at $ Pos last
+    \\ fs [])
+QED
+
+(* preservation of observable semantics *)
+
 Theorem semantics_attach_interpreter:
    semantics (ffi:'ffi ffi_state) max_app FEMPTY
      co (pure_cc (insert_interp ## I) cc) (attach_interpreter xs) <> Fail ==>
@@ -56,17 +211,32 @@ Proof
   strip_tac
   \\ ho_match_mp_tac IMP_semantics_eq \\ rw []
   \\ fs [] \\ fs [eval_sim_def] \\ rw []
-  \\ qmatch_asmsub_abbrev_tac ‘evaluate (_,_,iis) = _’
-  \\ qspecl_then [‘attach_interpreter xs’,‘[]’,‘iis’] mp_tac
-        (evaluate_interp_thm |> SIMP_RULE std_ss [] |> CONJUNCT1)
-  \\ disch_then drule \\ fs []
-  \\ disch_then $ qspec_then ‘initial_state ffi max_app
-        FEMPTY (pure_co (insert_interp ## I) ∘ co) cc k’ mp_tac
-  \\ impl_tac
-  >- simp [Abbr‘iis’,state_rel_def,initial_state_def]
-  \\ strip_tac \\ fs [closPropsTheory.initial_state_clock]
-  \\ first_x_assum $ irule_at $ Pos hd
-  \\ fs [state_rel_def]
+  \\ Cases_on ‘has_install_list xs’ \\ fs []
+  >-
+   (qmatch_asmsub_abbrev_tac ‘evaluate (_,_,iis) = _’
+    \\ qspecl_then [‘attach_interpreter xs’,‘[]’,‘iis’] mp_tac
+                   (evaluate_interp_thm |> SIMP_RULE std_ss [] |> CONJUNCT1)
+    \\ disch_then drule \\ fs []
+    \\ disch_then $ qspec_then ‘initial_state ffi max_app
+                                FEMPTY (pure_co (insert_interp ## I) ∘ co) cc k’ mp_tac
+    \\ impl_tac
+    >- simp [Abbr‘iis’,state_rel_def,initial_state_def]
+    \\ strip_tac \\ fs [closPropsTheory.initial_state_clock]
+    \\ first_x_assum $ irule_at $ Pos hd
+    \\ fs [state_rel_def])
+  >-
+   (qmatch_asmsub_abbrev_tac ‘evaluate (_,_,iis) = _’
+    \\ qspecl_then [‘attach_interpreter xs’,‘[]’,‘iis’] mp_tac
+                   (evaluate_change_oracle |> SIMP_RULE std_ss [] |> CONJUNCT1)
+    \\ fs []
+    \\ disch_then $ qspec_then ‘initial_state ffi max_app
+                                FEMPTY (pure_co (insert_interp ## I) ∘ co) cc k’ mp_tac
+    \\ impl_tac
+    >- (simp [Abbr‘iis’,state_rel'_def,initial_state_def,FEVERY_FEMPTY]
+        \\ fs [attach_interpreter_def,has_install_def] \\ EVAL_TAC)
+    \\ strip_tac \\ fs [closPropsTheory.initial_state_clock]
+    \\ qexists_tac ‘0’ \\ fs []
+    \\ fs [state_rel'_def])
 QED
 
 Theorem elist_globals_insert_interp:
